Core.v
@@ -3,4 +3,3 @@ From Elo Require Export Array.
 From Elo Require Export Map.
 From Elo Require Export Sem.
 From Elo Require Export SemExt.
-
