CriticalRegion.v
@@ -1,0 +1,234 @@
+From Elo Require Import Core.
+
+From Elo Require Import WellTypedTerm.
+
+(* ------------------------------------------------------------------------- *)
+(* insideCR                                                                  *)
+(* ------------------------------------------------------------------------- *)
+
+(* Ignores spawn blocks. *)
+Inductive insideCR (ad : addr) : tm -> Prop :=
+  | icr_fun : forall x Tx t,
+    insideCR ad t ->
+    insideCR ad <{fn x Tx t}>
+
+  | icr_call1 : forall t1 t2,
+    insideCR ad t1 ->
+    insideCR ad <{call t1 t2}>
+
+  | icr_call2 : forall t1 t2,
+    insideCR ad t2 ->
+    insideCR ad <{call t1 t2}>
+
+  | icr_new : forall T t,
+    insideCR ad t ->
+    insideCR ad <{new t : T}>
+
+  | icr_load : forall t,
+    insideCR ad t ->
+    insideCR ad <{*t}>
+
+  | icr_asg1 : forall t1 t2,
+    insideCR ad t1 ->
+    insideCR ad <{t1 := t2}>
+
+  | icr_asg2 : forall t1 t2,
+    insideCR ad t2 ->
+    insideCR ad <{t1 := t2}>
+
+  | icr_acq1 : forall t1 t2,
+    insideCR ad t1 ->
+    insideCR ad <{acq t1 t2}>
+
+  | icr_acq2 : forall t1 t2,
+    insideCR ad t2 ->
+    insideCR ad <{acq t1 t2}>
+
+  | icr_cr_eq : forall t,
+    insideCR ad <{cr ad t}>
+
+  | icr_cr_neq : forall ad' t,
+    ad <> ad' ->
+    insideCR ad t ->
+    insideCR ad <{cr ad' t}>
+  .
+
+(* ------------------------------------------------------------------------- *)
+(* tactics                                                                   *)
+(* ------------------------------------------------------------------------- *)
+
+Local Ltac _icr tt :=
+  match goal with
+  | H : insideCR _ <{unit     }> |- _ => tt H
+  | H : insideCR _ <{nat _    }> |- _ => tt H
+  | H : insideCR _ <{var _    }> |- _ => tt H
+  | H : insideCR _ <{fn _ _ _ }> |- _ => tt H
+  | H : insideCR _ <{call _ _ }> |- _ => tt H
+  | H : insideCR _ <{& _ : _  }> |- _ => tt H
+  | H : insideCR _ <{new _ : _}> |- _ => tt H
+  | H : insideCR _ <{* _      }> |- _ => tt H
+  | H : insideCR _ <{_ := _   }> |- _ => tt H
+  | H : insideCR _ <{acq _ _  }> |- _ => tt H
+  | H : insideCR _ <{cr _ _   }> |- _ => tt H
+  | H : insideCR _ <{spawn _  }> |- _ => tt H
+  end.
+
+Ltac inv_icr  := _icr inv.
+Ltac invc_icr := _icr invc.
+
+Local Ltac _value tt :=
+  match goal with
+  (* irrelevant for unit and nat *)
+  | H : value <{var _    }> |- _ => tt H
+  (* irrelevant for function *)
+  | H : value <{call _ _ }> |- _ => tt H
+  (* irrelevant for reference *)
+  | H : value <{new _ : _}> |- _ => tt H
+  | H : value <{* _      }> |- _ => tt H
+  | H : value <{_ := _   }> |- _ => tt H
+  | H : value <{acq _ _  }> |- _ => tt H
+  | H : value <{cr _ _   }> |- _ => tt H
+  | H : value <{spawn _  }> |- _ => tt H
+  end.
+
+Ltac inv_value  := _value inv.
+Ltac invc_value := _value invc.
+
+(* ------------------------------------------------------------------------- *)
+(* value-icr                                                                 *)
+(* ------------------------------------------------------------------------- *)
+
+Definition value_icr t := forall ad, value t -> ~ insideCR ad t.
+
+Local Lemma vicr_preservation_none : forall t1 t2,
+  value_icr t1 ->
+  t1 --[e_none]--> t2 ->
+  value_icr t2.
+Proof.
+  unfold value_icr. intros * Hvicr **.
+  ind_tstep.
+  - invc_value.
+  - invc_value.
+  - admit.
+  - invc_value.
+  - invc_value.
+  - invc_value.
+  - invc_value.
+  - invc_value.
+  - invc_value.
+  - admit.
+Qed.
+
+
+(* ------------------------------------------------------------------------- *)
+(* insideCR inheritance                                                          *)
+(* ------------------------------------------------------------------------- *)
+
+Local Lemma icr_inheritance_subst : forall ad x Tx t tx,
+  insideCR ad <{[x := tx] t}> ->
+  insideCR ad <{call <{fn x Tx t}> tx}>.
+Proof.
+  intros. induction t; eauto; simpl in *;
+  try (destruct str_eq_dec; subst; eauto using insideCR);
+  invc_icr; repeat auto_specialize; repeat invc_icr; eauto using insideCR.
+Qed.
+
+Local Lemma icr_inheritance_none : forall t1 t2 ad,
+  insideCR ad t2 ->
+  t1 --[e_none]--> t2 ->
+  insideCR ad t1.
+Proof.
+  intros. ind_tstep; try invc_icr; eauto using icr_inheritance_subst, insideCR.
+Qed.
+
+(* ------------------------------------------------------------------------- *)
+(* insideCR preservation                                                         *)
+(* ------------------------------------------------------------------------- *)
+
+Local Lemma icr_subst : forall t tx ad x,
+  insideCR ad t ->
+  insideCR ad <{[x := tx] t}>.
+Proof.
+  intros. induction t; eauto; simpl in *;
+  try (destruct str_eq_dec; subst); invc_icr; eauto using insideCR.
+Qed.
+
+Local Lemma icr_preservation_none : forall t1 t2 ad,
+  well_typed_term t1 ->
+  insideCR ad t1 ->
+  t1 --[e_none]--> t2 ->
+  insideCR ad t2.
+Proof.
+  intros. ind_tstep; invc_wtt; repeat invc_icr; eauto using insideCR.
+  - eauto using icr_subst.
+  - invc H0; invc_icr. admit.
+Qed.
+
+
+(* ------------------------------------------------------------------------- *)
+(* invariant                                                                 *)
+(* ------------------------------------------------------------------------- *)
+
+Definition critical_region_exclusivity (ths : threads) := forall ad tid1 tid2,
+  tid1 <> tid2 ->
+  insideCR ad ths[tid1] ->
+  ~ insideCR ad ths[tid2].
+
+(* ------------------------------------------------------------------------- *)
+(* preservation                                                              *)
+(* ------------------------------------------------------------------------- *)
+
+Local Lemma tstep_length_tid : forall ths tid e t,
+  ths[tid] --[e]--> t ->
+  tid < #ths.
+Proof.
+  intros.
+  decompose sum (lt_eq_lt_dec tid (#ths)); subst; sigma; eauto; invc_tstep.
+Qed.
+
+Local Ltac destruct_cre ths tid tid1 tid2 :=
+  assert (Hlt : tid < #ths) by eauto using tstep_length_tid;
+  destruct (nat_eq_dec tid tid1), (nat_eq_dec tid tid2); subst;
+  try contradiction.
+
+Local Lemma cre_preservation_none : forall t ths tid,
+  critical_region_exclusivity ths ->
+  ths[tid] --[e_none]--> t ->
+  critical_region_exclusivity ths[tid <- t].
+Proof.
+  unfold critical_region_exclusivity. intros.
+  destruct_cre ths tid tid1 tid2.
+  - sigma. eauto using icr_inheritance_none.
+  - sigma.
+
+  ind_tstep; intros ? ? ? Hneq Hicr;
+  repeat clean; repeat auto_specialize.
+  - admit.
+  - admit.
+  - admit.
+  - destruct (nat_eq_dec tid1 tid); destruct (nat_eq_dec tid2 tid); subst;
+    sigma; eauto.
+    + invc_icr. specialize (IHtstep ad tid tid2 Hneq). sigma. eauto.
+    + specialize (IHtstep ad tid1 tid Hneq). sigma. intros ?. invc_icr.
+      eapply IHtstep; eauto.
+
+
+
+
+  - intros ? ? ? Hneq Hicr.
+    repeat clean. repeat auto_specialize.
+    destruct (nat_eq_dec tid1 tid); destruct (nat_eq_dec tid2 tid); subst;
+    sigma; eauto.
+    + admit.
+    +
+
+
+      invc_icr.
+      * specialize (IHtstep ad tid2 tid1 Hneq). sigma.
+        intros ?. eapply IHtstep; eauto.
+      * eapply not_eq_sym in Hneq as Hneq1.
+        specialize (IHtstep ad tid1 tid2 Hneq1) as IH1. sigma.
+        eapply IH1. clear IH1.
+        specialize (IHtstep ad tid2 tid1 Hneq) as IH2. sigma.
+
+Qed.
