OldSafety.v
@@ -1,0 +1,257 @@
+From Coq Require Import Arith.Arith.
+From Coq Require Import Lists.List.
+From Coq Require Import Lia.
+
+From Elo Require Import Map.
+From Elo Require Import Properties.
+From Elo Require Import Lemmas.
+From Elo Require Import Preservation.
+From Elo Require Import PtrTyp.
+From Elo Require Import Soundness.
+From Elo Require Import Multistep.
+
+Local Lemma multistep_app : forall m1 m2 m3 ths1 ths2 ths3 tcA tcB,
+  m1 / ths1 ~~[tcA]~~>* m2 / ths2 ->
+  m2 / ths2 ~~[tcB]~~>* m3 / ths3 ->
+  m1 / ths1 ~~[tcB ++ tcA]~~>* m3 / ths3.
+Proof.
+  intros * ? Hmultistep. induction Hmultistep; eauto using multistep.
+Qed.
+
+Local Corollary multistep_append : forall m1 m2 m3 ths1 ths2 ths3 tid e tc,
+  m1 / ths1 ~~[tid, e]~~> m2 / ths2 ->
+  m2 / ths2 ~~[tc]~~>* m3 / ths3 ->
+  m1 / ths1 ~~[tc +++ (tid, e)]~~>* m3 / ths3.
+Proof.
+  eauto using multistep, multistep_app.
+Qed.
+
+Local Lemma destruct_multistep2 : forall tc m1 m3 ths1 ths3 tid e,
+  m1 / ths1  ~~[tc ++ (tid, e) :: nil]~~>* m3 / ths3 ->
+  (exists m2 ths2,
+    m1 / ths1 ~~[tid, e]~~> m2 / ths2 /\
+    m2 / ths2 ~~[tc]~~>*    m3 / ths3).
+Proof.
+  intros ?. induction tc; intros * Hmultistep; invc_mulst.
+  - inv_mulst. eauto using multistep.
+  - match goal with
+    | Hmultistep : _ / _ ~~[ _ ]~~>* _ / _ |- _ => 
+      decompose record (IHtc _ _ _ _ _ _ Hmultistep); eauto using multistep
+    end.
+Qed.
+
+Local Lemma destruct_multistep3 : forall tc m1 m4 ths1 ths4 tid1 tid2 e1 e2,
+  m1 / ths1  ~~[(tid2, e2) :: tc ++ (tid1, e1) :: nil]~~>* m4 / ths4 ->
+  (exists m2 ths2 m3 ths3,
+    m1 / ths1 ~~[tid1, e1]~~> m2 / ths2 /\
+    m2 / ths2 ~~[tc]~~>*      m3 / ths3 /\
+    m3 / ths3 ~~[tid2, e2]~~> m4 / ths4 ).
+Proof.
+  intros. invc_mulst.
+  match goal with H : _ / _ ~~[_]~~>* _ / _ |- _ =>
+    eapply destruct_multistep2 in H; decompose record H
+  end.
+  do 4 eexists. splits 3; eauto.
+Qed.
+
+(* ------------------------------------------------------------------------- *)
+(* TODO                                                                      *)
+(* ------------------------------------------------------------------------- *)
+
+Theorem nacc_preservation_multistep : forall m m' ths ths' tid ad tc,
+  valid_program m ths ->
+  (* --- *)
+  ad < #m ->
+  tid < #ths ->
+  ~ access ad m ths[tid] ->
+  m / ths ~~[tc]~~>* m' / ths' ->
+  ~ access ad m' ths'[tid].
+Proof.
+  intros. induction_mulst; eauto.
+  assert (#m   <= #m')   by eauto using multistep_nondecreasing_memory_length.
+  assert (#ths <= #ths') by eauto using multistep_nondecreasing_threads_length.
+  assert (valid_program m' ths') by eauto using vp_preservation.
+  eapply nacc_preservation in Hcstep; eauto with vp; try lia.
+Qed.
+
+Theorem spawned_thread_nacc_or_sacc : forall m m' ths ths' tid ad e,
+  forall_memory m (valid_addresses m) ->
+  forall_threads ths (valid_addresses m) ->
+  forall_threads ths well_typed_term ->
+  forall_threads ths safe_spawns ->
+  safe_memory_sharing m ths ->
+  (* --- *)
+  ad < #m ->
+  m / ths ~~[tid, e]~~> m' / ths' ->
+  ~ access ad m' ths'[#ths] \/ safe_access ad m' ths'[#ths].
+Proof.
+  intros. destruct (acc_dec ad m' ths'[#ths]); subst; eauto.
+  right. split; trivial. inv_cstep; simpl_array; eauto using spawn_nuacc.
+  intros ?. inv_uacc.
+Qed.
+
+Theorem nacc_or_sacc_cstep : forall m m' ths ths' tid tid' ad e,
+  forall_memory m (valid_addresses m) ->
+  forall_threads ths (valid_addresses m) ->
+  forall_threads ths well_typed_term ->
+  forall_threads ths safe_spawns ->
+  safe_memory_sharing m ths ->
+  (* --- *)
+  ad < #m ->
+  ~ access ad m ths[tid] ->
+  m / ths ~~[tid', e]~~> m' / ths' ->
+  (~ access ad m' ths'[tid]) \/ (tid = #ths /\ safe_access ad m' ths'[tid]).
+Proof.
+  intros. decompose sum (lt_eq_lt_dec tid (#ths)); subst; eauto.
+  - (* tid < #ths *)
+    eauto using nacc_preservation.
+  - (* tid = #ths *)
+    destruct (acc_dec ad m' ths'[#ths]); subst; eauto.
+    right. split; trivial.
+    inv_cstep; simpl_array; eauto using spawn_sacc. inv_acc.
+  - (* tid > #ths *)
+    destruct (nat_eq_dec tid tid'); subst; simpl_array;
+    inv_cstep; simpl_array; eauto with acc. inv_mstep; inv_tstep.
+Qed.
+
+Theorem nacc_or_sacc : forall m m' ths ths' tid ad tc,
+  valid_program m ths ->
+  (* --- *)
+  ad < #m ->
+  ~ access ad m ths[tid] ->
+  m / ths ~~[tc]~~>* m' / ths' ->
+  (~ access ad m' ths'[tid]) \/ (safe_access ad m' ths'[tid]).
+Proof.
+  intros * Hvp Hlt Hnacc **. induction_mulst; eauto.
+  assert (#m <= #m') by eauto using multistep_nondecreasing_memory_length.
+  assert (ad < #m') by lia.
+  assert (valid_program m' ths') by eauto using vp_preservation. 
+  destruct (IHmultistep Hvp Hlt Hnacc) as [? | [? ?]]; subst; clear IHmultistep.
+  - eapply nacc_or_sacc_cstep in Hcstep as [? | [_ ?]]; subst; eauto with vp.
+  - destruct (acc_dec ad m'' ths''[tid]); eauto. right. split; trivial.
+    eapply nuacc_preservation in Hcstep; eauto with vp.
+    decompose sum (lt_eq_lt_dec tid (#ths')); subst; trivial;
+    simpl_array; inv_acc.
+Qed.
+
+Theorem safety_write_read :
+  forall m m' ths ths' tid1 tid2 ad v1 v2 tc tc' T,
+    valid_program m ths ->
+    (* --- *)
+    tid1 <> tid2 ->
+    m / ths ~~[tc]~~>* m' / ths' ->
+    tc <> (tid2, EF_Read ad v2) :: tc' ++ (tid1, EF_Write ad v1 T) :: nil.
+Proof.
+  intros * Hvp Hneq Hmultistep Heq. rewrite Heq in Hmultistep.
+  specialize Hvp as H; destruct H as [_ [[_ ?] [[? ?] [[_ _] [_ Hsms]]]]].
+  rename m into m1. rename ths into ths1.
+  eapply destruct_multistep3 in Hmultistep
+    as [m2 [ths2 [m3 [ths3 [Hcstep1___ [Hmultistep Hcstep2___]]]]]].
+  (* --- *)
+  assert (valid_program m2 ths2) by eauto using vp_preservation. 
+  assert (valid_program m3 ths3) by eauto using vp_preservation. 
+  (* --- *)
+  assert (ad < #m1)
+    by eauto using vad_acc, write_requires_uacc, uacc_then_acc.
+  (* --- *)
+  assert (Hacc : access ad m3 ths3[tid2])
+    by eauto using read_requires_acc.
+  assert (Huacc : unsafe_access ad m1 ths1[tid1])
+    by eauto using write_requires_uacc.
+  assert (Hnacc : ~ access ad m1 ths1[tid2])
+    by (intros ?; eapply (Hsms tid1 tid2); eauto).
+  (* --- *)
+  assert (H' : m1 / ths1 ~~[tc' +++ (tid1, EF_Write ad v1 T)]~~>* m3 / ths3)
+    by eauto using multistep_append.
+  assert (m1[ad].typ = m3[ad].typ) by eauto using memtyp_preservation.
+  eapply nacc_or_sacc in H' as [? | ?]; eauto with vp.
+  eapply (ptyp_sacc_uacc_contradiction m3 m1 ths3[tid2] ths1[tid1]);
+  eauto with vp.
+Qed.
+
+Theorem safety_write_write :
+  forall m m' ths ths' tid1 tid2 ad v1 v2 tc tc' T1 T2,
+    valid_program m ths ->
+    (* --- *)
+    tid1 <> tid2 ->
+    m / ths ~~[tc]~~>* m' / ths' ->
+    tc <> (tid2, EF_Write ad v2 T2) :: tc' ++ (tid1, EF_Write ad v1 T1) :: nil.
+Proof.
+  intros * Hvp Hneq Hmultistep Heq. rewrite Heq in Hmultistep.
+  specialize Hvp as H; destruct H as [? [[? ?] [[? ?] [[? ?] [? Hsms]]]]].
+  rename m into m1. rename ths into ths1.
+  eapply destruct_multistep3 in Hmultistep
+    as [m2 [ths2 [m3 [ths3 [Hcstep1___ [Hmultistep Hcstep2___]]]]]].
+  (* --- *)
+  assert (valid_program m2 ths2) by eauto using vp_preservation. 
+  assert (Hvp3 : valid_program m3 ths3) by eauto using vp_preservation. 
+  destruct Hvp3 as [? [[? ?] [[? ?] [[? ?] [? Hsms3]]]]].
+  (* --- *)
+  assert (ad < #m1)
+    by eauto using vad_acc, write_requires_uacc, uacc_then_acc.
+  (* --- *)
+  assert (Huacc1 : unsafe_access ad m1 ths1[tid1])
+    by eauto using write_requires_uacc.
+  assert (Huacc3 : unsafe_access ad m3 ths3[tid2])
+    by (eapply write_requires_uacc; eauto; eapply des_vp_wtt; eauto).
+  assert (Hnacc : ~ access ad m1 ths1[tid2])
+    by (intros ?; eapply (Hsms tid1 tid2); eauto).
+  assert (Hnacc2 : ~ access ad m3 ths3[tid1])
+    by (intros ?; eapply (Hsms3 tid2 tid1); eauto).
+  (* --- *)
+  assert (H' : m1 / ths1 ~~[tc' +++ (tid1, EF_Write ad v1 T1)]~~>* m3 / ths3)
+    by eauto using multistep_append.
+  assert (m1[ad].typ = m3[ad].typ) by eauto using memtyp_preservation.
+  eapply nacc_or_sacc in H' as [? | ?];
+  eauto using uacc_then_acc.
+  eapply (ptyp_sacc_uacc_contradiction m3 m1 ths3[tid2] ths1[tid1]); eauto.
+Qed.
+
+(* TODO Need to clean this proof. *)
+Theorem safety_read_write :
+  forall m m' ths ths' tid1 tid2 ad v1 v2 tc tc' T,
+    valid_program m ths ->
+    (* --- *)
+    tid1 <> tid2 ->
+    m / ths ~~[tc]~~>* m' / ths' ->
+    tc <> (tid2, EF_Write ad v2 T) :: tc' ++ (tid1, EF_Read ad v1) :: nil.
+Proof.
+  intros * Hvp Hneq Hmultistep Heq. rewrite Heq in Hmultistep.
+  specialize Hvp as H; destruct H as [_ [[_ ?] [[? ?] [[_ _] [_ Hsms]]]]].
+  rename m into m1. rename ths into ths1.
+  eapply destruct_multistep3 in Hmultistep
+    as [m2 [ths2 [m3 [ths3 [Hcstep1___ [Hmultistep Hcstep2___]]]]]].
+  (* --- *)
+  assert (Hvp2 : valid_program m2 ths2) by eauto using vp_preservation. 
+  assert (Hvp3 : valid_program m3 ths3) by eauto using vp_preservation. 
+  (* --- *)
+  assert (ad < #m1) by eauto using vad_acc, read_requires_acc.
+  (* --- *)
+  assert (Huacc3 : unsafe_access ad m3 ths3[tid2])
+    by (eapply des_vp_wtt in Hvp3; eauto using write_requires_uacc).
+  (* --- *)
+  assert (Hdec : Decidable.decidable (unsafe_access ad m1 ths1[tid1]))
+    by eauto using uacc_dec.
+  destruct Hdec as [Huacc' | Hnuacc'].
+  - destruct Hvp3 as [? [[? ?] [[? ?] [[? ?] [? Hsms3]]]]].
+    assert (Hnacc : ~ access ad m1 ths1[tid2])
+      by (intros ?; eapply (Hsms tid1 tid2); eauto).
+    assert (Hnacc2 : ~ access ad m3 ths3[tid1])
+      by (intros ?; eapply (Hsms3 tid2 tid1); eauto).
+    assert (H' : m1 / ths1 ~~[tc' +++ (tid1, EF_Read ad v1)]~~>* m3 / ths3)
+      by eauto using multistep_append.
+    assert (m1[ad].typ = m3[ad].typ) by eauto using memtyp_preservation.
+    eapply nacc_or_sacc in H' as [? | ?];
+    eauto using uacc_then_acc.
+    eapply (ptyp_sacc_uacc_contradiction m3 m3 ths3[tid2] ths3[tid2]);
+    eauto with vp.
+  - assert (Hacc : access ad m1 ths1[tid1])
+      by eauto using read_requires_acc.
+    assert (Hsacc : safe_access ad m1 ths1[tid1]) by (split; eauto).
+    assert (H' : m1 / ths1 ~~[tc' +++ (tid1, EF_Read ad v1)]~~>* m3 / ths3)
+        by eauto using multistep_append.
+    assert (m1[ad].typ = m3[ad].typ) by eauto using memtyp_preservation.
+    eapply (ptyp_sacc_uacc_contradiction m1 m3 ths1[tid1] ths3[tid2]);
+    eauto with vp.
+Qed.
+
