SMS.v
@@ -1,0 +1,66 @@
+From Elo Require Import Core.
+
+From Elo Require Import Access.
+
+(* ------------------------------------------------------------------------- *)
+(* safe-memory-sharing                                                       *)
+(* ------------------------------------------------------------------------- *)
+
+Definition safe_memory_sharing m ths := forall tid1 tid2 ad,
+  tid1 <> tid2 ->
+  write_access ad m ths[tid1] ->
+  ~ write_access ad m ths[tid2].
+
+(* ------------------------------------------------------------------------- *)
+
+Local Lemma tstep_length_tid : forall ths tid e t,
+  ths[tid] --[e]--> t ->
+  tid < #ths.
+Proof.
+  intros.
+  decompose sum (lt_eq_lt_dec tid (#ths)); subst; sigma; eauto; invc_tstep.
+Qed.
+
+Local Ltac destruct_sms ths tid tid1 tid2 :=
+  assert (Hlt : tid < #ths) by eauto using tstep_length_tid;
+  destruct (nat_eq_dec tid tid1), (nat_eq_dec tid tid2); subst;
+  try contradiction.
+
+Lemma wacc_inheritance_subst : forall m x Tx t tx ad,
+  write_access ad m <{[x := tx] t}> ->
+  write_access ad m <{call <{fn x Tx t}> tx}>.
+Proof.
+  intros. induction t; eauto; simpl in *;
+  try (destruct str_eq_dec; subst; eauto using write_access);
+  invc_wacc; auto_specialize; repeat invc_wacc; eauto using write_access.
+Qed.
+
+Lemma wacc_inheritance_none : forall m t1 t2 ad,
+  write_access ad m t2 ->
+  t1 --[e_none]--> t2 ->
+  write_access ad m t1.
+Proof.
+  intros. ind_tstep; try inv_wacc;
+  eauto using wacc_inheritance_subst, write_access.
+Qed.
+
+Lemma nwacc_preservation_none : forall m t1 t2 ad,
+  ~ write_access ad m t1 ->
+  t1 --[e_none]--> t2 ->
+  ~ write_access ad m t2.
+Proof.
+  intros ** Hwacc.
+  ind_tstep. inv_nuacc; try inv_uacc; eauto.
+  inv_nuacc. contradict Huacc. eauto using (may_subst (unsafe_access ad)).
+Qed.
+
+Local Lemma sms_tstep_none_preservation : forall m t ths tid,
+  safe_memory_sharing m ths ->
+  ths[tid] --[e_none]--> t ->
+  safe_memory_sharing m ths[tid <- t].
+Proof.
+  intros ** tid1 tid2 **. destruct_sms ths tid tid1 tid2; sigma.
+  - eauto using wacc_inheritance_none.
+  - eauto using nwacc_preservation_none.
+  - admit.
+Qed.
